theories/Symbolic/GenOccursCheck.v
@@ -1,0 +1,663 @@
+(******************************************************************************)
+(* Copyright (c) 2019 Dominique Devriese, Georgy Lukyanov,                    *)
+(*   Sander Huyghebaert, Steven Keuchel                                       *)
+(* All rights reserved.                                                       *)
+(*                                                                            *)
+(* Redistribution and use in source and binary forms, with or without         *)
+(* modification, are permitted provided that the following conditions are     *)
+(* met:                                                                       *)
+(*                                                                            *)
+(* 1. Redistributions of source code must retain the above copyright notice,  *)
+(*    this list of conditions and the following disclaimer.                   *)
+(*                                                                            *)
+(* 2. Redistributions in binary form must reproduce the above copyright       *)
+(*    notice, this list of conditions and the following disclaimer in the     *)
+(*    documentation and/or other materials provided with the distribution.    *)
+(*                                                                            *)
+(* THIS SOFTWARE IS PROVIDED BY THE COPYRIGHT HOLDERS AND CONTRIBUTORS        *)
+(* "AS IS" AND ANY EXPRESS OR IMPLIED WARRANTIES, INCLUDING, BUT NOT LIMITED  *)
+(* TO, THE IMPLIED WARRANTIES OF MERCHANTABILITY AND FITNESS FOR A PARTICULAR *)
+(* PURPOSE ARE DISCLAIMED. IN NO EVENT SHALL THE COPYRIGHT HOLDER OR          *)
+(* CONTRIBUTORS BE LIABLE FOR ANY DIRECT, INDIRECT, INCIDENTAL, SPECIAL,      *)
+(* EXEMPLARY, OR CONSEQUENTIAL DAMAGES (INCLUDING, BUT NOT LIMITED TO,        *)
+(* PROCUREMENT OF SUBSTITUTE GOODS OR SERVICES; LOSS OF USE, DATA, OR         *)
+(* PROFITS; OR BUSINESS INTERRUPTION) HOWEVER CAUSED AND ON ANY THEORY OF     *)
+(* LIABILITY, WHETHER IN CONTRACT, STRICT LIABILITY, OR TORT (INCLUDING       *)
+(* NEGLIGENCE OR OTHERWISE) ARISING IN ANY WAY OUT OF THE USE OF THIS         *)
+(* SOFTWARE, EVEN IF ADVISED OF THE POSSIBILITY OF SUCH DAMAGE.               *)
+(******************************************************************************)
+
+From Equations Require Import
+     Equations.
+From Katamaran Require Import
+     Context
+     Environment
+     Notations
+     Prelude
+     Syntax.BinOps
+     Syntax.Terms
+     Syntax.TypeDecl
+     Syntax.Variables
+     Tactics.
+
+Import ctx.notations.
+Import env.notations.
+Import option.
+Import option.notations.
+
+Local Set Implicit Arguments.
+
+Module Type GenOccursCheckOn
+  (Import TY : Types)
+  (Import TM : TermsOn TY).
+
+  Local Notation LCtx := (NCtx LVar Ty).
+
+  Class SubstUniv (Sb : LCtx -> LCtx -> Type) :=
+    MkSubstUniv {
+        initSU : forall {Σ}, Sb [ctx] Σ
+      ; transSU : forall {Σ1 Σ2 Σ3}, Sb Σ1 Σ2 -> Sb Σ2 Σ3 -> Sb Σ1 Σ3
+      ; interpSU : forall {Σ1 Σ2}, Sb Σ1 Σ2 -> Sub Σ1 Σ2
+      }.
+
+  Class SubstSU (Sb : LCtx -> LCtx -> Type) (T : LCtx -> Type) :=
+    substSU : forall {Σ1 Σ2}, T Σ1 -> Sb Σ1 Σ2 -> T Σ2.
+
+  #[export] Instance substSubstSU `{SubstUniv Sb} `{Subst T} : SubstSU Sb T :=
+    fun {Σ1 Σ2} t σ => subst t (interpSU σ).
+
+  Class SubstUnivLaws Sb `{SubstUniv Sb} :=
+    interpTransSU : forall {Σ1 Σ2 Σ3} (σ1 : Sb Σ1 Σ2) (σ2 : Sb Σ2 Σ3),
+        interpSU (transSU σ1 σ2) = subst (interpSU σ1) (interpSU σ2).
+  Arguments SubstUnivLaws Sb {H}.
+
+  Class SubstSULaws Sb `{SubstSU Sb T} {su : SubstUniv Sb} {sul : SubstUnivLaws Sb} :=
+    substSU_trans : forall {Σ1 Σ2 Σ3} (σ1 : Sb Σ1 Σ2) (σ2 : Sb Σ2 Σ3) (t : T Σ1),
+        substSU t (transSU σ1 σ2) = substSU (substSU t σ1) σ2.
+  Arguments SubstSULaws Sb T {H su sul}.
+
+  #[export] Instance substSubstSULaws `{Subst T, SubstLaws T} `{SubstUnivLaws Sb}
+    : SubstSULaws Sb T.
+  Proof.
+    intros Σ1 Σ2 Σ3 σ1 σ2 t.
+    unfold substSU, substSubstSU.
+    now rewrite interpTransSU, subst_sub_comp.
+  Qed.
+
+  Record MeetResult `{SubstUniv Sb} Σ Σ1 Σ2 :=
+    MkMeetResult {
+        Σ12 : LCtx
+      ; meetLeft : Sb Σ1 Σ12
+      ; meetRight : Sb Σ2 Σ12
+      ; meetUp : Sb Σ12 Σ
+      }.
+
+  Class SubstUnivMeet Sb `{SubstUniv Sb} :=
+    meetSU : forall {Σ Σ1 Σ2} (σ1 : Sb Σ1 Σ) (σ2 : Sb Σ2 Σ), MeetResult Σ Σ1 Σ2
+  .
+  Arguments SubstUnivMeet Sb {H}.
+  Class SubstUnivMeetLaws Sb `{SubstUnivMeet Sb} :=
+    MkSubstUnivMeetLaws {
+        meetLeftCorrect : forall {Σ Σ1 Σ2} (σ1 : Sb Σ1 Σ) (σ2 : Sb Σ2 Σ),
+          transSU (meetLeft (meetSU σ1 σ2)) (meetUp (meetSU σ1 σ2)) = σ1
+      ; meetRightCorrect : forall {Σ Σ1 Σ2} (σ1 : Sb Σ1 Σ) (σ2 : Sb Σ2 Σ),
+          transSU (meetRight (meetSU σ1 σ2)) (meetUp (meetSU σ1 σ2)) = σ2
+      }.
+  Arguments SubstUnivMeetLaws Sb {H} {H0}.
+
+  Class SubstUnivVar `{SubstUnivMeet Sb} :=
+    suVar : forall {x Σ} (xIn : x ∈ Σ), Sb [ x ]%ctx  Σ.
+  Arguments SubstUnivVar Sb {H} {H0}.
+
+  Class SubstUnivVarUp `{SubstUnivVar Sb} :=
+    upSU : forall {Σ1 Σ2 x}, Sb Σ1 Σ2 -> Sb (Σ1 ▻ x) (Σ2 ▻ x)
+  .
+  Arguments SubstUnivVarUp Sb {H H0 H1}.
+
+  Class SubstUnivVarDown `{SubstUnivVar Sb} :=
+    MkSubstUnivVarDown {
+        wkVarSU : forall {Σ1 Σ2 x}, x ∈ Σ1 -> Sb Σ1 Σ2 -> x ∈ Σ2
+      ; downSU : forall {Σ1 Σ2 x} (xIn : x ∈ Σ1) (σ : Sb Σ1 Σ2),
+          let xIn' := wkVarSU xIn σ in Sb (Σ1 - x) (Σ2 - x)
+      }.
+  Arguments SubstUnivVarDown Sb {H H0 H1}.
+
+  Class SubstUnivVarLaws `{SubstUnivVar Sb} :=
+    suVarSound : forall `(xIn : x ∈ Σ), interpSU (suVar xIn) = [ term_var_in xIn ]%env.
+  Arguments SubstUnivVarLaws Sb {H} {H0} {H1}.
+
+  Class GenOccursCheck `{SubstUniv Sb} (T : LCtx -> Type) : Type :=
+    gen_occurs_check : forall {Σ} (t : T Σ), { Σ' & (Sb Σ' Σ * T Σ')%type }.
+
+  #[export] Instance GenOccursCheck_Const {Sb} {sSb : SubstUniv Sb} {A} : GenOccursCheck (Const A) :=
+    fun Σ v => existT _ (initSU (SubstUniv := sSb), v).
+  
+  #[export] Instance gen_occurs_check_env `{SubstUnivMeet Sb}
+    {I : Set} {T : LCtx -> I -> Set}
+    {sT : forall i : I, Subst (fun Σ : LCtx => T Σ i)}
+    {OCT : forall i, GenOccursCheck (fun Σ => T Σ i)} :
+    forall {Γ : Ctx I}, GenOccursCheck (fun Σ => Env (T Σ) Γ) :=
+    fix oc {Γ Σ} ts {struct ts} :=
+      match ts with
+      | env.nil         => existT [ctx] (initSU , [env])
+      | env.snoc ts _ t =>
+          let '(existT Σ1 (σ1 , ts')) := oc ts in
+          let '(existT Σ2 (σ2 , t')) := gen_occurs_check t in
+          let '(MkMeetResult _ _ _ _ Σ12 σ1' σ2' σ') := meetSU σ1 σ2 in
+          existT Σ12 (σ' ,
+                    (env.snoc (B := I) (substSU ts' σ1') _ (substSU t' σ2')))
+      end.
+
+  #[export] Instance gen_occurs_check_term `{SubstUnivVar Sb} :
+    forall σ, GenOccursCheck (fun Σ => Term Σ σ) :=
+    fix gen_occurs_check_term {τ Σ} (t : Term Σ τ) {struct t} :
+      { Σ' & (Sb Σ' Σ * Term Σ' τ)%type } :=
+      match t with
+      | term_var_in xIn => existT _ (suVar xIn , term_var_in ctx.in_zero)
+      | term_val σ v => existT [ctx] (initSU , term_val σ v)
+      | term_binop op t1 t2 =>
+          let '(existT Σ1 (σ1 , t1')) := gen_occurs_check_term t1 in
+          let '(existT Σ2 (σ2 , t2')) := gen_occurs_check_term t2 in
+          let '(MkMeetResult _ _ _ _ Σ12 σ1' σ2' σ') := meetSU σ1 σ2 in
+          (existT Σ12 (σ' , term_binop op (substSU t1' σ1') (substSU t2' σ2')))
+      | term_unop op t =>
+          let '(existT Σ1 (σ1 , t')) := gen_occurs_check_term t in
+          (existT Σ1 (σ1 , term_unop op t'))
+      | term_tuple ts =>
+        let '(existT Σ1 (σ1 , ts')) := gen_occurs_check_env (OCT := @gen_occurs_check_term) ts in
+        (existT Σ1 (σ1 , term_tuple ts'))
+      | term_union U K t0 =>
+          let '(existT Σ1 (σ1 , ts')) := gen_occurs_check_term t0 in
+          (existT Σ1 (σ1 , term_union U K ts'))
+      | term_record R ts =>
+        let OCTerm xt := @gen_occurs_check_term (@type recordf Ty xt) in
+        let '(existT Σ1 (σ1 , ts')) := gen_occurs_check_env (OCT := OCTerm) ts in
+        (existT Σ1 (σ1 , term_record R ts'))
+      end.
+
+  #[export] Instance gen_occurs_check_list `{SubstUnivMeet Sb} {T : LCtx -> Type} {sT : Subst T} `{ocT : GenOccursCheck Sb T} :
+    GenOccursCheck (List T) :=
+    fix oc {Σ} ls {struct ls} :=
+      match ls with
+      | nil => (existT [ctx] (initSU , nil))
+      | (l :: ls)%list => let '(existT Σ1 (σ1 , l')) := gen_occurs_check l in
+                          let '(existT Σ2 (σ2 , ls')) := oc ls in
+                          let '(MkMeetResult _ _ _ _ Σ12 σ1' σ2' σ') := meetSU σ1 σ2 in
+                          (existT Σ12 (σ' ,
+                                    cons (substSU l' σ1') (substSU ls' σ2')))
+      end.
+
+  #[export] Instance gen_occurs_check_pair `{SubstUnivMeet Sb} `{GenOccursCheck Sb AT, GenOccursCheck Sb BT, Subst AT, Subst BT} :
+    GenOccursCheck (Pair AT BT) :=
+    fun _ '(a,b) =>
+      let '(existT Σ1 (σ1 , a')) := gen_occurs_check a  in
+      let '(existT Σ2 (σ2 , b')) := gen_occurs_check b  in
+      let '(MkMeetResult _ _ _ _ Σ12 σ1' σ2' σ') := meetSU σ1 σ2 in
+      (existT Σ12 (σ' , (substSU a' σ1', substSU b' σ2'))).
+
+  #[export] Instance gen_occurs_check_option `{SubstUniv Sb} {AT} `{GenOccursCheck Sb AT} :
+    GenOccursCheck (Option AT) :=
+    fun _ ma =>
+      match ma with
+      | Some a => let '(existT Σ1 (σ1 , a')) := gen_occurs_check a in
+                  (existT Σ1 (σ1 , Some a'))
+      | None   => (existT [ctx] (initSU , None))
+      end.
+
+  #[export] Instance gen_occurscheck_ctx `{SubstUnivMeet Sb} {A} {sA : Subst A} {ocA : GenOccursCheck A} :
+    GenOccursCheck (fun Σ => Ctx (A Σ)) :=
+    fix oc {Σ} ys {struct ys} :=
+      match ys with
+      | ctx.nil       => (existT [ctx] (initSU , ctx.nil))
+      | ctx.snoc ys y => let '(existT Σ1 (σ1 , ys')) := oc ys  in
+                         let '(existT Σ2 (σ2 , y'))  := ocA _ y in
+                         let '(MkMeetResult _ _ _ _ Σ12 σ1' σ2' σ') := meetSU σ1 σ2 in
+                         (existT Σ12 (σ' , ctx.snoc (substSU ys' σ1') (substSU y' σ2')))
+      end.
+
+  Class GenOccursCheckLaws `{sSb : SubstUniv Sb}
+    (T : LCtx -> Type)  {ocT : GenOccursCheck T} {sT : Subst T} : Type :=
+    MkGenOccursCheckLaws {
+       oc_sound : forall {Σ} (t : T Σ),
+          let '(existT Σ' (σ , t')) := gen_occurs_check t in
+          substSU t' σ = t
+      }.
+  Arguments GenOccursCheckLaws {Sb} {sSb} T {ocT} {sT}.
+
+  (* Hm, I seem to need something more... *)
+  (* Lemma oc_univ {Sb} {sSb : SubstUnivMeet Sb} *)
+  (*   (T : LCtx -> Type) {sT : Subst T} {_ : GenOccursCheckLaws T} *)
+  (*   {Σ1 Σ} {σ : Sb Σ1 Σ} {t : T Σ1} : *)
+  (*   let '(existT Σ1' (σ1 , ts')) := (gen_occurs_check (subst t (interpSU σ))) in *)
+  (*   exists σt, σ = transSU σt σ1. *)
+  (* Proof. *)
+  (*   generalize (oc_sound (subst t (interpSU σ))). *)
+  (*   destruct (gen_occurs_check (subst t (interpSU σ))) as (Σ' & (σ' , t')). *)
+  (*   destruct (meetSU σ' σ) as [Σ12 σ1' σ2' σ'' corrσ1' corrσ2']. *)
+  (*   rewrite <- corrσ1', <-corrσ2'. *)
+  (*   rewrite ?interpTransSU. *)
+  (* Abort.  *)
+
+  (* TODO: automate proofs... *)
+  (* Ltac occurs_check_mixin := *)
+  (*   match goal with *)
+  (*   | H: ?P |- ?P => exact H *)
+  (*   | |- ?x = ?x => refine eq_refl *)
+  (*   | |- ?x = ?y => *)
+  (*       let hx := head x in *)
+  (*       let hy := head y in *)
+  (*       is_constructor hx; is_constructor hy; *)
+  (*       first [ subst; refine eq_refl (* | f_equal *) ] *)
+  (*   | |- wlp _ (occurs_check ?xIn ?t) => *)
+  (*       generalize (occurs_check_sound xIn t); *)
+  (*       apply wlp_monotonic; intros ? -> *)
+  (*   | |- wp _ (occurs_check ?xIn (subst ?t _)) => *)
+  (*       generalize (occurs_check_shift xIn t); *)
+  (*       apply wp_monotonic; intros ? := *)
+  (*   | |- OccursCheckLaws _ => *)
+  (*       constructor; unfold OccursCheckShiftPoint, OccursCheckSoundPoint; *)
+  (*       let x := fresh in *)
+  (*       intros ? ? ? x; induction x *)
+  (*   end. *)
+
+  (* Ltac occurs_check_derive := *)
+  (*   repeat *)
+  (*     (try progress cbn; *)
+  (*      first *)
+  (*        [ option.tactics.mixin *)
+  (*        | occurs_check_mixin]); *)
+  (*   try progress cbn; try easy. *)
+  (* Local Ltac derive := occurs_check_derive. *)
+
+  #[export, refine] Instance gen_occurs_check_laws_env `{SubstUnivVar Sb} {_ : SubstUnivLaws Sb} {_ : SubstUnivMeetLaws Sb}
+    {I : Set} {T : LCtx -> I -> Set}
+    {sT : forall i : I, Subst (fun Σ : LCtx => T Σ i)}
+    {slT : forall i : I, SubstLaws (fun Σ : LCtx => T Σ i)}
+    {OCT : forall i, GenOccursCheck (Sb := Sb) (fun Σ => T Σ i)}
+    {OCTL : forall i, GenOccursCheckLaws (Sb := Sb) (fun Σ => T Σ i) } :
+    forall {Γ : Ctx I}, GenOccursCheckLaws (Sb := Sb) (fun Σ => Env (T Σ) Γ) :=
+    fun {Γ} => MkGenOccursCheckLaws _ _ _.
+  Proof.
+    induction t; first easy.
+    cbn.
+    change (gen_occurs_check_env t) with (gen_occurs_check (T := fun Σ => Env (T Σ) Γ) t).
+    destruct (gen_occurs_check t) as (Σ1 & σ1 & t').
+    generalize (oc_sound db).
+    destruct (gen_occurs_check db) as (Σ2 & σ2 & db').
+    intros Hdb.
+    generalize (meetLeftCorrect σ1 σ2).
+    generalize (meetRightCorrect σ1 σ2).
+    destruct (meetSU σ1 σ2) as [Σ12 σ1' σ2' σ']; cbn -[subst].
+    intros corrσ1 corrσ2.
+    change (substSU (?x ► (?b ↦ ?xs))%env ?σ) with (substSU x σ ► (b ↦ substSU xs σ)).
+    now rewrite <-?substSU_trans, corrσ1, corrσ2 , IHt, Hdb.
+  Qed.
+
+  #[export,refine] Instance gen_occurs_check_laws_term `{SubstUnivVarLaws Sb} {_ : SubstUnivLaws Sb} {_ : SubstUnivMeetLaws Sb} {τ} :
+    GenOccursCheckLaws (fun Σ => Term Σ τ) :=
+    MkGenOccursCheckLaws _ _ _.
+  Proof.
+    induction t; cbn.
+    - now rewrite (suVarSound lIn).
+    - easy.
+    - revert IHt1 IHt2.
+      change (gen_occurs_check_term ?t) with (gen_occurs_check (T := fun Σ => Term Σ _) t).
+      destruct (gen_occurs_check t1) as (Σ1 & ς1 & t1').
+      destruct (gen_occurs_check t2) as (Σ2 & ς2 & t2').
+      generalize (meetLeftCorrect ς1 ς2).
+      generalize (meetRightCorrect ς1 ς2).
+      destruct (meetSU ς1 ς2) as [Σ12 ς1' ς2' ς]; cbn -[subst].
+      intros  corrς1' corrς2'.
+      intros Ht1 Ht2.
+      change (substSU (term_binop ?op ?t1 ?t2) ?σ) with (term_binop op (substSU t1 σ) (substSU t2 σ)).
+      now rewrite <-?substSU_trans, corrς1', corrς2', Ht1, Ht2.
+    - revert IHt.
+      change (gen_occurs_check_term ?t) with (gen_occurs_check (T := fun Σ => Term Σ _) t).
+      destruct (gen_occurs_check t) as (Σ' & ς & t').
+      now intros <-.
+    - change (gen_occurs_check_env ?t) with (gen_occurs_check (T := fun Σ => Env (Term Σ) _) t).
+      cut (let '(existT Σ' (σ, ts')) := gen_occurs_check ts in substSU (T := fun Σ => Env (Term Σ) _) ts' σ = ts).
+      + destruct (gen_occurs_check ts) as (Σ1 & σ1 & t').
+        now intros <-.
+      + induction IH; first easy.
+        cbn.
+        change (gen_occurs_check_env ?t) with (gen_occurs_check (T := fun Σ => Env (Term Σ) _)t).
+        destruct (gen_occurs_check E) as (Σ1 & σ1 & env').
+        destruct (gen_occurs_check d) as (Σ2 & σ2 & d').
+        generalize (meetLeftCorrect σ1 σ2).
+        generalize (meetRightCorrect σ1 σ2).
+        destruct (meetSU σ1 σ2) as [Σ12 σ1' σ2' σ']; cbn -[subst].
+        intros  corrσ1 corrσ2.
+        change (substSU ((?x ► (?b ↦ ?xs))%env) ?σ) with (substSU x σ ► (b ↦ substSU xs σ)).
+        now rewrite <-?substSU_trans, corrσ1, corrσ2, IHIH, q.
+    - change (gen_occurs_check_term ?t) with (gen_occurs_check (T := fun Σ => Term Σ _) t).
+      destruct (gen_occurs_check t) as (Σ' & ς & t').
+      change (substSU (term_union ?U ?K ?t) ?σ) with (term_union U K (substSU t σ)).
+      now rewrite IHt.
+    - change (gen_occurs_check_env ?t) with (gen_occurs_check (T := fun Σ => NamedEnv (Term Σ) _) t).
+      cut (let '(existT Σ' (σ, ts')) := gen_occurs_check ts in substSU (T := fun Σ => NamedEnv (Term Σ) _) ts' σ = ts).
+      + destruct (gen_occurs_check ts) as (Σ1 & σ1 & t').
+        now intros <-.
+      + induction IH; first easy.
+        cbn.
+        change (gen_occurs_check_env ?t) with (gen_occurs_check (T := fun Σ => Env (fun b => Term Σ _) _) t).
+        destruct (gen_occurs_check E) as (Σ1 & σ1 & env').
+        destruct (gen_occurs_check d) as (Σ2 & σ2 & d').
+        generalize (meetLeftCorrect σ1 σ2).
+        generalize (meetRightCorrect σ1 σ2).
+        destruct (meetSU σ1 σ2) as [Σ12 σ1' σ2' σ']; cbn -[subst NamedEnv].
+        intros  corrσ1 corrσ2.
+        change (substSU ((?x ► (?b ↦ ?xs))%env) ?σ) with (substSU x σ ► (b ↦ substSU xs σ)).
+        change (substSU env' σ1 = E) in IHIH.
+        now rewrite <-?substSU_trans, corrσ1, corrσ2, q, IHIH.
+  Qed.
+
+  #[export,refine] Instance gen_occurs_check_laws_list `{SubstUnivMeet Sb} {_ : SubstUnivLaws Sb} {_ : SubstUnivMeetLaws Sb}
+     `{SubstLaws T} {_ : GenOccursCheck T} {_ : GenOccursCheckLaws T} :
+    GenOccursCheckLaws (List T) :=
+    MkGenOccursCheckLaws _ _ _.
+  Proof.
+    induction t; first easy.
+    cbn.
+    generalize (oc_sound a).
+    destruct (gen_occurs_check a) as (Σ1 & σ1 & a').
+    intros <-.
+    destruct (gen_occurs_check t) as (Σ2 & σ2 & t').
+    generalize (meetLeftCorrect σ1 σ2).
+    generalize (meetRightCorrect σ1 σ2).
+    destruct (meetSU σ1 σ2) as [Σ12 σ1' σ2' σ']; cbn -[subst].
+    intros  corrσ1 corrσ2.
+    change (substSU (?x :: ?xs)%list ?σ) with (substSU x σ :: substSU xs σ)%list.
+    now rewrite <-?substSU_trans, corrσ1, corrσ2, IHt.
+  Qed.
+
+  #[export] Instance gen_occurs_check_laws_sub `{SubstUnivVarLaws Sb} {_ : SubstUnivLaws Sb} {_ : SubstUnivMeetLaws Sb} {Σ} :
+    GenOccursCheckLaws (Sub Σ) :=
+    gen_occurs_check_laws_env.
+
+  #[export,refine] Instance gen_occurs_check_laws_pair `{SubstUnivMeet Sb, SubstLaws AT, SubstLaws BT} {_ : SubstUnivLaws Sb} {_ : SubstUnivMeetLaws Sb}
+    {_ : GenOccursCheck AT} {_ : GenOccursCheckLaws AT}
+    {_ : GenOccursCheck BT} {_ : GenOccursCheckLaws BT} :
+    GenOccursCheckLaws (Pair AT BT) :=
+    MkGenOccursCheckLaws _ _ _.
+  Proof.
+    destruct t.
+    cbn.
+    generalize (oc_sound a).
+    destruct (gen_occurs_check a) as (Σ1 & σ1 & a').
+    generalize (oc_sound b).
+    destruct (gen_occurs_check b) as (Σ2 & σ2 & b').
+    generalize (meetLeftCorrect σ1 σ2).
+    generalize (meetRightCorrect σ1 σ2).
+    destruct (meetSU σ1 σ2) as [Σ12 σ1' σ2' σ']; cbn -[subst].
+    intros corrσ1 corrσ2.
+    change (substSU (?x , ?xs) ?σ) with (substSU x σ , substSU xs σ).
+    rewrite <-?substSU_trans, corrσ1, corrσ2.
+    now intros -> ->.
+  Qed.
+
+  #[export,refine] Instance gen_occurs_check_laws_option `{SubstUnivMeet Sb, SubstLaws AT} {_ : GenOccursCheck AT} {_ : GenOccursCheckLaws AT} :
+    GenOccursCheckLaws (Option AT) :=
+    MkGenOccursCheckLaws _ _ _.
+  Proof.
+    induction t; last easy.
+    cbn.
+    generalize (oc_sound a).
+    destruct (gen_occurs_check a) as (Σ1 & σ1 & a').
+    change (substSU (Some ?x) ?σ) with (Some (substSU x σ))%list.
+    now intros ->.
+  Qed.
+
+  #[export] Instance gen_occurs_check_unit `{SubstUniv Sb} : GenOccursCheck Unit :=
+    fun _ t => match t with tt => (existT [ctx] (initSU , tt)) end.
+
+  #[export,refine] Instance gen_occurs_check_laws_unit `{SubstUniv Sb} :
+    GenOccursCheckLaws Unit :=
+    MkGenOccursCheckLaws _ _ _.
+  Proof.
+    now destruct t.
+  Qed.
+
+  #[export,refine] Instance gen_occurscheck_laws_ctx `{SubstUnivMeet Sb} {_ : SubstUnivLaws Sb} {_ : SubstUnivMeetLaws Sb}
+    `{SubstLaws A} {_ :GenOccursCheck A} {_ :GenOccursCheckLaws A} :
+    GenOccursCheckLaws (fun Σ => Ctx (A Σ)) :=
+    MkGenOccursCheckLaws _ _ _.
+  Proof.
+    induction t; first easy.
+    cbn.
+    destruct (gen_occurs_check t) as (Σ1 & σ1 & a').
+    generalize (oc_sound b).
+    change (g _ ?t) with (gen_occurs_check t).
+    destruct (gen_occurs_check b) as (Σ2 & σ2 & b').
+    generalize (meetLeftCorrect σ1 σ2).
+    generalize (meetRightCorrect σ1 σ2).
+    destruct (meetSU σ1 σ2) as [Σ12 σ1' σ2' σ']; cbn -[subst].
+    intros corrσ1 corrσ2.
+    change (substSU (?x ▻ ?xs) ?σ) with (substSU x σ ▻ substSU xs σ).
+    rewrite <-?substSU_trans, corrσ1, corrσ2, IHt.
+    now intros ->.
+  Qed.
+
+  Section Weakenings.
+    Inductive WeakensTo : LCtx -> LCtx -> Set :=
+    | WkNil : WeakensTo [ctx] [ctx]
+    | WkSkipVar : forall {Σ1 Σ2} x, WeakensTo Σ1 Σ2 -> WeakensTo Σ1 (Σ2 ▻ x)
+    | WkKeepVar : forall {Σ1 Σ2} x, WeakensTo Σ1 Σ2 -> WeakensTo (Σ1 ▻ x) (Σ2 ▻ x)
+    .
+
+    Fixpoint interpWk {Σ1 Σ2} (wk : WeakensTo Σ1 Σ2) : Sub Σ1 Σ2 :=
+      match wk with
+      | WkNil => [env]
+      | WkSkipVar x wk => subst (interpWk wk) sub_wk1
+      | WkKeepVar x wk => sub_up1 (interpWk wk)
+      end.
+
+    Equations transWk {Σ1 Σ2 Σ3} (wk12 : WeakensTo Σ1 Σ2) (wk23 : WeakensTo Σ2 Σ3) : WeakensTo Σ1 Σ3 :=
+    | wk1 | WkSkipVar _ wk2 => WkSkipVar _ (transWk wk1 wk2)
+    | WkNil | wk2 => wk2
+    | WkSkipVar x wk1 | WkKeepVar _ wk2 => WkSkipVar _ (transWk wk1 wk2)
+    | WkKeepVar x wk1 | WkKeepVar _ wk2 => WkKeepVar _ (transWk wk1 wk2)
+    .
+
+    Lemma interpTransWk {Σ1 Σ2 Σ3} (wk12 : WeakensTo Σ1 Σ2) (wk23 : WeakensTo Σ2 Σ3) :
+      interpWk (transWk wk12 wk23) = subst (interpWk wk12) (interpWk wk23).
+    Proof.
+      eapply (transWk_elim (fun Σ1 Σ2 Σ3 wk12 wk23 wk13 => interpWk wk13 = subst (Subst := SubstEnv) (interpWk wk12) (interpWk wk23)));
+        cbn -[subst].
+      - now intros.
+      - intros * ->.
+        apply sub_comp_assoc.
+      - intros * ->.
+        rewrite !(sub_comp_assoc (interpWk wk1)).
+        now rewrite sub_comp_wk1_comm.
+      - intros * ->.
+        apply sub_up1_comp.
+    Defined.
+
+    Fixpoint wkNilInit {Σ} : WeakensTo [ctx] Σ :=
+      match Σ with
+      | [ctx] => WkNil
+      | Σ ▻ x => WkSkipVar x wkNilInit
+      end.
+
+    Fixpoint wkRefl {Σ} : WeakensTo Σ Σ :=
+      match Σ with
+      | [ctx] => WkNil
+      | Σ ▻ x => WkKeepVar x wkRefl
+      end.
+
+    Inductive WeakenZeroView Σ2 b : forall Σ1, WeakensTo Σ1 (Σ2 ▻ b) -> Type :=
+    | VarUnused : forall Σ1 (wk : WeakensTo Σ1 Σ2), WeakenZeroView (WkSkipVar b wk)
+    | VarUsed : forall Σ1 (wk : WeakensTo Σ1 Σ2), WeakenZeroView (WkKeepVar b wk)
+    .
+
+    Equations weakenZeroView {Σ1 Σ2 b} (wk : WeakensTo Σ1 (Σ2 ▻ b)) : WeakenZeroView wk :=
+    | WkSkipVar _ wk => VarUnused b wk
+    | WkKeepVar _ wk => VarUsed b wk
+    .
+
+    Fixpoint wkRemove (Σ : LCtx) b (bIn : b ∈ Σ) : WeakensTo (Σ - b) Σ :=
+      ctx.In_case (fun b Σ bIn => WeakensTo (Σ - b) Σ)
+                  (fun b Σ => WkSkipVar _ wkRefl)
+                  (fun b' Σ b bIn => WkKeepVar _ (wkRemove bIn))
+                  bIn.
+
+    Fixpoint wkSingleton {Σ : LCtx} {b} (bIn : b ∈ Σ) : WeakensTo [ b ]%ctx Σ :=
+      ctx.In_case (fun b Σ bIn => WeakensTo [ b ]%ctx Σ)
+                  (fun b Σ => WkKeepVar _ wkNilInit)
+                  (fun b' Σ b bIn => WkSkipVar _ (wkSingleton bIn))
+                  bIn.
+
+    Equations wkVarZeroIn {Σ Σ' : LCtx} {b} (σ : WeakensTo (Σ' ▻ b)%ctx Σ) : b ∈ Σ :=
+    | WkKeepVar _ _ => ctx.in_zero
+    | WkSkipVar _ wk => ctx.in_succ (wkVarZeroIn wk)
+    .
+
+    Fixpoint weakenIn {Σ1 Σ2 : LCtx} (σ : WeakensTo Σ1 Σ2) : forall {b} (bIn : b ∈ Σ1), b ∈ Σ2 :=
+      match σ with
+      | WkNil => fun b (bIn : b ∈ [ctx]) => match ctx.view bIn with end
+      | WkSkipVar _ σ' => fun b bIn => ctx.in_succ (weakenIn σ' bIn)
+      | WkKeepVar _ σ' => fun b bIn => match ctx.view bIn with
+                                     | ctx.isZero => ctx.in_zero
+                                     | ctx.isSucc bIn' => ctx.in_succ (weakenIn σ' bIn')
+                                     end
+      end.
+
+    Lemma weakenRemovePres {Σ1 Σ2} (wk : WeakensTo Σ1 Σ2) :
+      forall {b} (bIn : b ∈ Σ1),
+        let bIn' := weakenIn wk bIn in WeakensTo (Σ1 - b) (Σ2 - b).
+    Proof.
+      induction wk; intros b bIn.
+      - destruct (ctx.view bIn).
+      - apply WkSkipVar, IHwk.
+      - destruct (ctx.view bIn); first easy.
+        apply WkKeepVar, IHwk.
+    Defined.
+
+    Inductive WeakenRemoveView {Σ b} : forall {Σ1} (bIn : b ∈ Σ), WeakensTo Σ1 (Σ - b) -> Set :=
+    | MkWeakenRemoveView : forall Σ1' (bIn' : b ∈ Σ1') (σ1' : WeakensTo Σ1' Σ), WeakenRemoveView (weakenIn σ1' bIn') (weakenRemovePres σ1' bIn').
+
+    Definition weakenRemoveView : forall {b Σ} (bIn : b ∈ Σ) Σ1 (σ : WeakensTo Σ1 (Σ - b)), WeakenRemoveView bIn σ :=
+        ctx.In_rect (fun b Σ bIn => forall Σ1 σ, WeakenRemoveView bIn σ)
+                  (fun b Σ Σ1 σ => MkWeakenRemoveView ctx.in_zero (WkKeepVar _ σ))
+                  (fun b Σ b' bIn IHbIn Σ1 σ =>
+                     match weakenZeroView σ with
+                     | VarUsed _ σ' =>
+                         match IHbIn _ σ'
+                               in WeakenRemoveView bIn σ'
+                               return WeakenRemoveView (ctx.in_succ bIn) _ with
+                         | (MkWeakenRemoveView bIn' σ1') =>
+                             MkWeakenRemoveView (ctx.in_succ bIn') (WkKeepVar _ σ1')
+                         end
+                     | VarUnused _ σ' =>
+                         match IHbIn _ σ'
+                               in WeakenRemoveView bIn σ'
+                               return WeakenRemoveView (ctx.in_succ bIn) _ with
+                         | MkWeakenRemoveView bIn' σ1' =>
+                             MkWeakenRemoveView bIn' (WkSkipVar _ σ1')
+                         end
+                     end
+                  ).
+
+    #[export] Instance substUniv_weaken : SubstUniv WeakensTo.
+    Proof.
+      econstructor.
+      - intros. exact wkNilInit.
+      - intros. eapply transWk; eassumption.
+      - intros; now eapply interpWk.
+    Defined.
+
+    Definition extendMeetSkipSkip {Σ1 Σ2 Σ3 x} (meet : MeetResult Σ3 Σ1 Σ2) :
+      MeetResult (Σ3 ▻ x) Σ1 Σ2 :=
+      match meet with
+        MkMeetResult _ _ _ _ Σ12 σ1' σ2' σ' => MkMeetResult _ _ _ _ Σ12 σ1' σ2' (WkSkipVar x σ')
+      end.
+    Definition extendMeetSkipKeep {Σ1 Σ2 Σ3 x} (meet : MeetResult Σ3 Σ1 Σ2) :
+      MeetResult (Σ3 ▻ x) Σ1 (Σ2 ▻ x) :=
+      match meet with
+        MkMeetResult _ _ _ _ Σ12 σ1' σ2' σ' => MkMeetResult _ _ _ _ _ (WkSkipVar x σ1') (WkKeepVar _ σ2') (WkKeepVar x σ')
+      end.
+    Definition extendMeetKeepSkip {Σ1 Σ2 Σ3 x} (meet : MeetResult Σ3 Σ1 Σ2) :
+      MeetResult (Σ3 ▻ x) (Σ1 ▻ x) Σ2 :=
+      match meet with
+        MkMeetResult _ _ _ _ Σ12 σ1' σ2' σ' => MkMeetResult _ _ _ _ _ (WkKeepVar x σ1') (WkSkipVar _ σ2') (WkKeepVar x σ')
+      end.
+    Definition extendMeetKeepKeep {Σ1 Σ2 Σ3 x} (meet : MeetResult Σ3 Σ1 Σ2) :
+      MeetResult (Σ3 ▻ x) (Σ1 ▻ x) (Σ2 ▻ x) :=
+      match meet with
+        MkMeetResult _ _ _ _ Σ12 σ1' σ2' σ'  => MkMeetResult _ _ _ _ _ (WkKeepVar x σ1') (WkKeepVar _ σ2') (WkKeepVar x σ')
+      end.
+    Equations meetWk {Σ1 Σ2 Σ3} (wk13 : WeakensTo Σ1 Σ3) (wk23 : WeakensTo Σ2 Σ3) :
+      MeetResult Σ3 Σ1 Σ2 :=
+    | WkNil | WkNil => MkMeetResult _ _ _ _ _ WkNil WkNil WkNil
+    | WkSkipVar x wk1 | WkSkipVar _ wk2 => extendMeetSkipSkip (meetWk wk1 wk2)
+    | WkSkipVar x wk1 | WkKeepVar _ wk2 => extendMeetSkipKeep (meetWk wk1 wk2)
+    | WkKeepVar x wk1 | WkSkipVar _ wk2 => extendMeetKeepSkip (meetWk wk1 wk2)
+    | WkKeepVar x wk1 | WkKeepVar _ wk2 => extendMeetKeepKeep (meetWk wk1 wk2)
+    .
+
+    #[export] Instance substUnivMeet_weaken : SubstUnivMeet WeakensTo :=
+      fun _ _ _ => meetWk.
+    #[export] Instance substUnivMeetLaws_weaken : SubstUnivMeetLaws WeakensTo.
+    Proof.
+      constructor; intros.
+      - apply (meetWk_elim (fun _ _ _ wk1 wk2 res => transSU (meetLeft res) (meetUp res) = wk1));
+        cbn; first reflexivity; intros;
+        destruct (meetWk wk1 wk2) as [Σ12 σ1' σ2' σ']; cbn in *;
+          rewrite ?transWk_equation_2, ?transWk_equation_3, ?transWk_equation_4;
+          now f_equal.
+      - apply (meetWk_elim (fun _ _ _ wk1 wk2 res => transSU (meetRight res) (meetUp res) = wk2));
+        cbn; first reflexivity; intros;
+        destruct (meetWk wk1 wk2) as [Σ12 σ1' σ2' σ']; cbn in *;
+          rewrite ?transWk_equation_2, ?transWk_equation_3, ?transWk_equation_4;
+          now f_equal.
+    Qed.
+
+    Definition wkVar : forall {x Σ}, x ∈ Σ -> WeakensTo [ x ]%ctx Σ :=
+      ctx.In_rect (fun x Σ xIn => WeakensTo [ x ]%ctx Σ)
+                  (fun x Σ => WkKeepVar x wkNilInit)
+                  (fun x Σ y xIn wk => WkSkipVar y wk).
+
+    Lemma interpWk_wkVar : forall {x Σ} {xIn : x ∈ Σ},
+      interpWk (wkVar xIn) = [ term_var_in xIn ]%env.
+    Proof.
+      eapply ctx.In_ind.
+      - intros.
+        refine (f_equal (fun x => x.[b ↦ _]) _).
+        match goal with |- ?env = [env] => now destruct (env.view env) end.
+      - intros.
+        change (interpWk (wkVar (ctx.in_succ bIn))) with
+                 (subst (interpWk (wkVar bIn)) (sub_wk1 (b := b'))).
+        rewrite H.
+        cbn.
+        now rewrite lookup_sub_wk1.
+    Qed.
+
+    #[export] Instance substUnivVar_weaken : SubstUnivVar WeakensTo :=
+      (fun x Σ xIn => wkVar xIn).
+    #[export] Instance substUnivVarUp_weaken : SubstUnivVarUp WeakensTo.
+    Proof.
+      intros Σ1 Σ2 x σ; now eapply WkKeepVar.
+    Defined.
+    #[export] Instance substUnivVarDown_weaken : SubstUnivVarDown WeakensTo.
+    Proof.
+      refine (MkSubstUnivVarDown _ (fun _ _ _ xIn σ => weakenIn σ xIn) _).
+      intros; eapply weakenRemovePres.
+    Defined.
+
+    #[export] Instance substUnivVarLaws_weaken : SubstUnivVarLaws WeakensTo :=
+      (fun _ _ xIn => interpWk_wkVar).
+
+    Fixpoint restrictEnv {D} {Σ1 Σ2 : LCtx} (wk : WeakensTo Σ1 Σ2) :
+      Env D Σ2 -> Env D Σ1.
+    Proof.
+      induction wk; first easy.
+      intros e. eapply IHwk, env.tail. now eassumption.
+      intros e. destruct (env.view e) as [e v].
+      apply env.snoc; last easy.
+      now eapply IHwk.
+    Qed.
+
+  End Weakenings.
+
+End GenOccursCheckOn.
